# Chapter 3

## 3.1

First, we observe that:

* When n = 1, the output is 1. This is the base case.
* When n = 2, the output is 4.
* When n = 3, the output is 9.

Induction hypothesis. Suppose `\sum_{i=0}^{n-1}(2i+1) = n^2`.

Induction step. For `n + 1`, we need to prove that `\sum_{i=0}^{n}(2i+1) = (n+1)^2`.

    \sum_{i=0}^{n}
        = \sum_{i=0}^{n-1} + (2n+1)
        = n^2 + (2n+1)
        = (n+1)^2

## 3.2

First, let's restate the principle based on count(Y). For every n >= 1, it is true that

    For any finit sets X and Y such that count(X) > count(Y) and count(Y) = n, if f is a map from X to Y, then there are distinct elements x_1, x_2 in X, y in Y,  such that f(x_1) = f(x_2) = y.

Base case. n = 1. If count(X) > count(Y), we suppose count(X) = 2. Since there is a function from X to Y, both elements in X must be mapped to the only element in Y.

Induction hypothesis. Suppose for some n >= 1, count(X) > count(Y), count(Y) = n, and f is a function from X to Y, there are two discinct elements in X, and another element in Y, such that f(x_1) = f(x_2) = y.

Induction step. We need to prove that if count(Y) = n+1, there are two distinct elements in X, and another element in Y, such that f(x_1) = f(x_2) = y.

Case 1. For an element y in Y, if it is mapped by two distinct elements in X, the induction is proved.

Case 2. If such y is mapped by only one element in X, we take it away from Y. Now count(Y) = n and count(X) > count(Y). This is exactly our hypothesis.

## 3.3

The Extended Pigeon Hole Principle states that if count(X) > k*count(Y), and there is a map f from X to Y, it is true that there are at least k+1 elements in X, such that f(x_1) = f(x_2) = ... = f(x_{k+1})

Base case. When k=1, we can use the Pigeon Hole Principle to prove this situation.

Induction hypothesis. Suppose for a certain k>1, if count(X) > k*count(Y), and there is a map f from X to Y, it is true that there are at least k+1 elements in X, such that f(x_1) = f(x_2) = ... = f(x_{k+1})

Induction step. We need to prove that if count(X) > (k+1) * count(Y), there are at least k+2 elements in X, and all of them are mapped to the same element in Y.
Note that count(X) + count(Y) > (k+1) * count(Y). It means that we add count(Y) distinct elements to the existing X set.

Case 1. There are at least one newly added element x, which satisfies that f(x_1) = f(x). By adding this element to our existing k+1 elements, we have k+2 elements in X that are mapped to the same element in Y.

Case 2. None of the newly added elements is mapped to the same element in Y as x_1. Now let's create two new sets, X' and Y'. For X', first we remove k+1 elements (x_1, x_2, ... , x_{k+1}) from X. Then we add count(Y) new elements. Therefore, count(X') = count(X) - (k+1) + count(Y). For Y, we remove the element y that is mapped by k+1 elments in X. So count(Y') = count(Y)-1.

    count(X') - count(Y')
    = (count(X) - (k+1) + count(Y)) - (count(Y)-1)
    = count(X)-k
    > k*count(Y)-k      // According to our hypothesis, count(X) > k*count(Y).
    = k*(count(Y)-1)
    = k*count(Y')       // By definition, count(Y') = count(Y)-1

This shows that count(X') > (k+1) * count(Y'). According to our hypothesis, there are at least k+2 elements in X' which are all mapped to the same element in Y'.

## 3.4

### (a)

\sum_{i=0}^{n-1}(2^{2i+1})

Base case. When n=1, 2/3 * (4^1-1) = 2.

Induction hypothesis. Suppose for an integer k>1,

    \sum_{i=0}^{k-1}(2^{2i+1}) = 2/3 * (4^k-1)

Induction step. We need to prove that,

    \sum_{i=0}^{k}(2^{2i+1}) = 2/3 * (4^(k+1)-1)

Proof.

    \sum_{i=0}^{k}(2^{2i+1})
    = \sum_{i=0}^{k-1}(2^{2i+1}) + 2^{2k+1}
    = 2/3 * (4^k-1) + 2^{2k+1}
    = 2/3 * (4^k-1) + 2*4^k
    = 2/3 * (4^k-1 + 3*4^k)
    = 2/3 * (4^(k+1)-1)

### (b)

    \prod_{i=1}^{n}(2^{-i})
    = 2^{-(1+2+3+...+n)}
    = 2^{-(n*(n+1))/2}

## 3.5

Base case. When n=0, \sum_{i=0}^{n}(i^2) = 0.

Induction hypothesis. Suppose for k>0,

    \sum_{i=0}^{k}(i^2) = \frac{k*(k+1)*(2k+1)}{6}

Induction step. We need to prove that,

    \sum_{i=0}^{k+1}(i^2) = \frac{(k+1)*(k+2)*(2k+3)}{6}

Proof.

    \sum_{i=0}^{k+1}(i^2)
    = \sum_{i=0}^{k}(i^2) + (k+1)^2
    = \frac{k * (k+1) * (2k+1)}{6} + (k+1)^2
    = \frac{k * (k+1) * (2k+1) + 6*(k+1)^2}{6}
    = \frac{(k+1) * (k*(2k+1) + 6(k+1))}{6}
    = \frac{(k+1) * (2k^2+7k+6)}{6}
    = \frac{(k+1) * (k+2) * (2k+3)}{6}

## 3.6






## 3.1

## 3.1

## 3.1

## 3.1

## 3.1

## 3.1

## 3.1

## 3.1

## 3.1

## 3.1

