# Chapter 8

## 8.1

Base case: If s is an empty string, #_a(s) = 0.

Constructor case: Let s = <b, s'>, n = 0. If a == b, n += 1. Repeat this step until we reach the base case. #_a(s) = n.

Proof.

When both s and t are empty strings,

    #_a(s) = #_a(\lambda) = 0   (1)
    #_a(t) = #_a(\lambda) = 0   (2)

According to the base case in 8.3,

    #_a(s \dot t)
    = #_a(\lambda \dot \lambda)
    = #_a(\lambda) = 0          (3)

Therefore, (3) = (1) + (2).

Suppose #_a(s \dot t) = #_a(s) + #_a(t). Let s' = <p, s>, t' = <q, t>, where p and q are characters. According to our constructor case,

    #_a(s') = #_a(p) + #_a(s)   (4)
    #_a(t') = #_a(q) + #_a(t)   (5)

According to 8.3,

    #_a(s' \dot t')
    = #_a(<p, s> \dot t')
    = #_a(<p, s \dot t'>)
    = #_a(p) + #_a(s \dot t')   (6)

Let s \dot t' = <s_i, s_j> \dot t' = <s_i, s_j \dot t'>, where s_i is a character and s_j is a string by removing s_i from s. Since the sum of all #_a(s_i) is equal to #_a(s),

    (6)
    = #_a(p) + #_a(s) + #_a(<q, t>)
    = #_a(p) + #_a(s) + #_a(q) + #_a(t)     (7)

It turns out that (7) = (4) + (5)

## 8.2

### (a)

Base case: The reverse of an empty string is the empty string itself.

Constructor case: Let x = <u, v>. x^R = v^R \dot u.

### (b)

If both u and v are empty strings, the equation holds. Now let u' = <p, u>, v' = <q, v>.

    v'^R \dot u'^R
    = <q, v>^R \dot <p, u>^R
    = (v^R \dot q) \dot (u^R \dot p)        (1)

    (u' \dot v')^R
    = (<p, u> \dot v')^R
    = (<p, u \dot v'>)^R
    = (u \dot v')^R \dot p                  (2)

Let u = <x, y>, where x is a character and y is a string.

    (u \dot v')^R
    = (<x, y> \dot v')^R
    = <x, y \dot v'>^R
    = (y \dot v')^R \dot x              // Constructor case.
    = ((y \dot q) \dot v)^R \dot x
    = v^R \dot (y \dot q)^R \dot x      // Induction hypothesis.
    = v^R \dot q \dot y^R \dot x
    = v^R \dot q \dot u^R               (3)

By replacing part of (2) by (3), we have (2) = (1).

### (c)

Suppose ((x^R))^R = x. Let x' = <s, x>.

    (<s, x>^R)^R
    = (x^R \dot s)^R
    = s \dot ((x^R))^R      // According to 8.2(b).
    = s \dot x
    = x'

## 8.3

Prove that if a binary string is a hedgehog, it has equal numbers of 0s and 1s.

First, an empty string is a hedgehog and it has zero 0 and 1. Second, suppose h is a hedgehog and it has equal 0s and 1s. We cannot generate another hedgehog by adding one digit to h. We need to add at least two digits, a 0 and a 1, following either rule 2, 3 or 4 to create a new hedgehog g. It turns out that g also has equal numbers of 0s and 1s.

Prove that if a binary string has equal numbers of 0s and 1s, it is a hedgehog.

According to the statement, the length of the binary string is an even number 2N. Therefore we can cut the string into N segments. Each segment has exactly 2 digits. Every segment can be one of four combinations: 01, 10, 00 and 11.

If all segments are either 10 or 01, obviously the string is a hedgehog. Otherwise reduce the string by removing segments from both ends. Keep reducing if the removed segment is either 01 or 10. When we have a combination of 00 or 11 on one end, there must be a 11 or 00 on the other end because: (1) 0s and 1s must be of the same amount for the original string; (2) We have already removed equal numbers of 0s and 1s. We can remove these 11 and 00 in pairs as the reverse step of rule 2 or 3. The removement stops until we have an empty string left. These are the reverse steps of building a hedgehog.

## 8.4

If both u and v are empty strings, the length of u, v and u \dot v are 0. The equation holds. Suppose for string u and v of length m and n,

    |u \dot v| = |u| + |v|

Let u' = <x, u>, v' = <y, v>, where x and y are characters.

    |u'| + |v'|
    = |<x, u>| + |<y, v>|
    = |u| + 1 + |v| + 1     // According to the definition of string length.
    = |u| + |v| + 2         (1)

    |u' \dot v'|
    = |<x, u> \dot v'|
    = |<x, u \dot v'>|
    = |u \dot v'| + 1       (2)

Let u = <x_i, u_i>, where x_i is a character and u_i is a string.

    |u \dot v'|
    = |<x_i, u_i> \dot v'|
    = |<x_i, u_i \dot v'>|
    = |u_i \dot v'| + 1     (3)

Repeat the procedure above m times, note that m is the length of string u, we have

    (3)
    = |v'| + |u|
    = |<y, v>| + |u|
    = |v| + 1 + |u|         (4)

Replace part of (2) with (4), it turns out that (2) = (1).

## 8.5

Consider the constructor cases of BSP. If a BSP is created by C1 only, it has the form (((x))), which is exactly what the statement requires. If such a BSP is created by C1 and C2, for example, (x)(y), there are two cases.

If both x and y are contructed solely by C1, by replacing the only `)(` into `()`, we have (x()y). If either x or y is construced by C2, let x = (u)(v). Do the replacement recursively until both u and v are constructed by C1. In this way we transform a BSP into a string that meets the requirement.

## 8.6

### (a)

Weight 0: 0.

Weight 1: <0, 0>.

Weight 2: <0, <0, 0>>, <<0, 0>, 0>.

Weight 3:

    <0, <0, <0, 0>>>, <<0, <0, 0>>, 0>,
    <0, <<0, 0>, 0>>, <<<0, 0>, 0>, 0>,
    <<0, 0>, <0, 0>>.

### (b)

When n = 0, t must be 0, so h(0) = 0, the statement is true. Suppose for width n, the inequations hold.

Let t_{n+1} = <t_n, 0>. h(t_{n+1}) = 1+h(t) <= n+1.

Let t_{n+1} = <t_p, t_q>, where p >= q and p+q = n+1. Therefore

    h(t_{n+1}) = 1+h(p)

The maximum possible p is when n is an odd number 2k+1, p=k.

    h(t_{n+1})
    = 1 + h(p)
    >= 1 + h(k)
    = 1 + ceil(lg(k + 1))
    = ceil(lg(2k + 2))
    = ceil(lg(n + 1))

We can generate t_{n+1} following two ways mentioned above so that they meet the lower and upper bounds.

## 8.7

Unknown.

## 8.8

Base case. SS(<a, \lambda>) = {\lambda, a}

Constructor case. Let s' = <a, s>. SS(s') = union(SS(s), {<a, b>: b are all the elements in SS(s)}).
